SeparationLogic/ProofTheory/IterSepcon.v
@@ -1,0 +1,86 @@
+Require Import Coq.Classes.Morphisms.
+Require Import Coq.Classes.RelationClasses.
+Require Import Coq.Logic.Classical_Prop.
+Require Import Coq.Sorting.Permutation.
+Require Import Logic.lib.Coqlib.
+Require Import Logic.lib.List_Func_ext.
+Require Import Logic.GeneralLogic.Base.
+Require Import Logic.MinimunLogic.Syntax.
+Require Import Logic.PropositionalLogic.Syntax.
+Require Import Logic.SeparationLogic.Syntax.
+Require Import Logic.MinimunLogic.ProofTheory.Normal.
+Require Import Logic.MinimunLogic.ProofTheory.Minimun.
+Require Import Logic.MinimunLogic.ProofTheory.RewriteClass.
+Require Import Logic.MinimunLogic.ProofTheory.ContextProperty.
+Require Import Logic.PropositionalLogic.ProofTheory.Intuitionistic.
+Require Import Logic.PropositionalLogic.ProofTheory.WeakClassical.
+Require Import Logic.PropositionalLogic.ProofTheory.GodelDummett.
+Require Import Logic.PropositionalLogic.ProofTheory.Classical.
+Require Import Logic.PropositionalLogic.ProofTheory.RewriteClass.
+Require Import Logic.SeparationLogic.ProofTheory.SeparationLogic.
+Require Import Logic.SeparationLogic.ProofTheory.RewriteClass.
+Require Import Logic.SeparationLogic.ProofTheory.DerivedRules.
+
+Local Open Scope logic_base.
+Local Open Scope syntax.
+Import PropositionalLanguageNotation.
+Import SeparationLogicNotation.
+
+Definition iter_sepcon' {L: Language} {nL: NormalLanguage L} {pL: PropositionalLanguage L} {sL: SeparationLanguage L} (default: expr) (xs: list expr) : expr := semi_group_fold default sepcon xs.
+
+Definition iter_sepcon {L: Language} {nL: NormalLanguage L} {pL: PropositionalLanguage L} {sL: SeparationLanguage L} {s'L: SeparationEmpLanguage L} (xs: list expr) : expr := iter_sepcon' emp xs.
+
+Definition iter_wand {L: Language} {nL: NormalLanguage L} {pL: PropositionalLanguage L} {sL: SeparationLanguage L} {s'L: SeparationEmpLanguage L} (xs: list expr) (y: expr) : expr := fold_right wand y xs.
+
+Lemma sepcon_iter_sepcon' {L: Language} {nL: NormalLanguage L} {pL: PropositionalLanguage L} {sL: SeparationLanguage L} {Gamma: ProofTheory L} {nGamma: NormalProofTheory L Gamma} {mpGamma: MinimunPropositionalLogic L Gamma} {ipGamma: IntuitionisticPropositionalLogic L Gamma} {sGamma: SeparationLogic L Gamma}:
+  forall (default: expr) x xs y ys,
+    |-- iter_sepcon' default (x :: xs) * iter_sepcon' default (y :: ys) <-->
+        iter_sepcon' default ((x :: xs) ++ (y :: ys)).
+Proof.
+  intros.
+  apply (@Equivalence_Symmetric _ _ provable_iffp_equiv).
+  apply (@semi_group_fold_app expr _ provable_iffp_equiv sepcon sepcon_proper_iffp default).
+  + intros.
+    apply (@Equivalence_Symmetric _ _ provable_iffp_equiv).
+    apply sepcon_assoc.
+  + intro; congruence.
+  + intro; congruence.
+Qed.
+
+Lemma sepcon_iter_sepcon {L: Language} {nL: NormalLanguage L} {pL: PropositionalLanguage L} {sL: SeparationLanguage L} {s'L: SeparationEmpLanguage L} {Gamma: ProofTheory L} {nGamma: NormalProofTheory L Gamma} {mpGamma: MinimunPropositionalLogic L Gamma} {ipGamma: IntuitionisticPropositionalLogic L Gamma} {sGamma: SeparationLogic L Gamma} {EmpGamma: EmpSeparationLogic L Gamma}:
+  forall xs ys,
+    |-- iter_sepcon xs * iter_sepcon ys <--> iter_sepcon (xs ++ ys).
+Proof.
+  intros.
+  destruct xs as [| x xs], ys as [| y ys].
+  + simpl.
+    apply sepcon_emp.
+  + simpl.
+    rewrite provable_sepcon_comm_iffp.
+    apply sepcon_emp.
+  + simpl.
+    rewrite app_nil_r.
+    apply sepcon_emp.
+  + apply sepcon_iter_sepcon'.
+Qed.
+
+Instance proper_iter_sepcon'_iffp {L: Language} {nL: NormalLanguage L} {pL: PropositionalLanguage L} {sL: SeparationLanguage L} {Gamma: ProofTheory L} {nGamma: NormalProofTheory L Gamma} {mpGamma: MinimunPropositionalLogic L Gamma} {ipGamma: IntuitionisticPropositionalLogic L Gamma} {sGamma: SeparationLogic L Gamma} (default: expr):
+  Proper (Forall2 (fun x y => |-- iffp x y) ==> (fun x y => |-- iffp x y)) (iter_sepcon' default).
+Proof.
+  intros.
+  apply proper_semi_group_fold.
+  apply sepcon_proper_iffp.
+Qed.
+
+Instance proper_iter_sepcon'_Permutation {L: Language} {nL: NormalLanguage L} {pL: PropositionalLanguage L} {sL: SeparationLanguage L} {Gamma: ProofTheory L} {nGamma: NormalProofTheory L Gamma} {mpGamma: MinimunPropositionalLogic L Gamma} {ipGamma: IntuitionisticPropositionalLogic L Gamma} {sGamma: SeparationLogic L Gamma} (default: expr):
+  Proper (@Permutation expr ==> (fun x y => |-- iffp x y)) (iter_sepcon' default).
+Proof.
+  intros.
+  hnf; intros.
+  apply (@comm_semi_group_fold_perm expr _ provable_iffp_equiv sepcon sepcon_proper_iffp default); auto.
+  + intros.
+    apply provable_sepcon_comm_iffp.
+  + intros.
+    apply (@Equivalence_Symmetric _ _ provable_iffp_equiv).
+    apply sepcon_assoc.
+Qed.
